BSWLean/Treelike.lean
@@ -20,8 +20,71 @@ abbrev TreeLikeRefutation {vars} (φ : CNFFormula vars) :=
 class Unsat {vars} (f : CNFFormula vars) : Prop where
   h_unsat : ∀ a, f.eval a = false
 
-lemma tree_like_proof_is_correct {vars} {φ : CNFFormula vars} (c : Clause vars) (h_c_in_φ : c ∈ φ)
+lemma tree_like_proof_is_correct {vars} {φ : CNFFormula vars} (c : Clause vars)
     (π : TreeLikeResolution φ c) : ∀ a, φ.eval a → c.eval a := by
   intro a h_φ_eval_a
   rw [CNFFormula.eval_eq_true_iff_all_satisfied_clauses] at h_φ_eval_a
-  sorry
+  induction π
+  case axiom_clause h_c_in_φ =>
+    (expose_names; exact h_φ_eval_a c_1 h_c_in_φ)
+  case weakening c' h_c'_subset_c π' ih =>
+    expose_names
+    rw [Clause.eval_eq_true_iff_exists_satisfied_literal]
+    rw [Clause.eval_eq_true_iff_exists_satisfied_literal] at ih
+    obtain ⟨l, h_l_in_c', h_l_eval_a⟩ := ih
+    use l
+    constructor
+    · exact h_c'_subset_c h_l_in_c'
+    · exact h_l_eval_a
+  case resolve c₁ c₂ v h_v_mem_vars h_v_not_mem_c π₁ π₂ h_resolve ih₁ ih₂ =>
+    expose_names
+    rw [Clause.eval_eq_true_iff_exists_satisfied_literal]
+    rw [Clause.eval_eq_true_iff_exists_satisfied_literal] at ih₁
+    rw [Clause.eval_eq_true_iff_exists_satisfied_literal] at ih₂
+    by_cases a v h_v_mem_vars
+    case neg h =>
+      obtain ⟨l₁, h_l₁_in_c₁, h_l₁_eval_a⟩ := ih₁
+      rw [←h_resolve.left] at h_l₁_in_c₁
+      use l₁
+      simp only [h_l₁_eval_a, and_true]
+      contrapose! h_l₁_in_c₁
+      simp only [Finset.union_singleton, Finset.mem_insert, h_l₁_in_c₁, or_false]
+      suffices l₁.eval a ≠ (v.toLiteral h_v_mem_vars).eval a by
+        contrapose! this
+        simp only [this]
+      rw [h_l₁_eval_a]
+      unfold Literal.eval
+      unfold Variable.toLiteral
+      simp only [ne_eq, Bool.true_eq, Bool.not_eq_true]
+      exact eq_false_of_ne_true h
+    case pos h =>
+      obtain ⟨l₂, h_l₂_in_c₂, h_l₂_eval_a⟩ := ih₂
+      rw [←h_resolve.right] at h_l₂_in_c₂
+      use l₂
+      simp only [h_l₂_eval_a, and_true]
+      contrapose! h_l₂_in_c₂
+      simp only [Finset.union_singleton, Finset.mem_insert, h_l₂_in_c₂, or_false]
+      suffices l₂.eval a ≠ (v.toNegLiteral h_v_mem_vars).eval a by
+        contrapose! this
+        simp only [this]
+      rw [h_l₂_eval_a]
+      unfold Literal.eval
+      unfold Variable.toNegLiteral
+      simp only [ne_eq, Bool.true_eq, Bool.not_eq_true]
+      exact Bool.not_eq_eq_eq_not.mpr h
+
+
+theorem tree_like_refutation_implies_unsat {vars} {φ : CNFFormula vars}
+    (π : TreeLikeRefutation φ) : Unsat φ := by
+  unfold TreeLikeRefutation at π
+  apply tree_like_proof_is_correct at π
+  have : ∀ a : Assignment vars, BotClause.eval a = false := by
+    unfold Clause.eval
+    unfold BotClause
+    exact fun a ↦ rfl
+  constructor
+  intro a
+  by_contra! h
+  simp only [ne_eq, Bool.not_eq_false] at h
+  apply π a at h
+  contradiction
